[typing] cleaner apply_spec implementation. Problem, extraction fails

template-coq/theories/AstUtils.v
@@ -2,7 +2,7 @@ From Coq Require Import Ascii String Bool OrderedType Lia List Program Arith.
 From Template Require Import Ast utils.
 Import List.ListNotations.
 Require Import FunctionalExtensionality.
-Require Import ssreflect.
+Require Import ssreflect ssrbool ssrfun.
 
 Set Asymmetric Patterns.
 
@@ -176,22 +176,22 @@ Definition eq_projection p p' :=
   let '(ind', pars', arg') := p' in
   eq_ind ind ind' && eq_nat pars pars' && eq_nat arg arg'.
 
-Lemma eq_string_refl x : eq_string x x = true.
+Lemma eq_string_refl x : eq_string x x.
 Proof.
   unfold eq_string.
   now rewrite (proj2 (string_compare_eq x x) eq_refl).
 Qed.
 
-Lemma eq_ind_refl i : eq_ind i i = true.
+Lemma eq_ind_refl i : eq_ind i i.
 Proof.
   destruct i as [mind k].
   unfold eq_ind. now rewrite eq_string_refl Nat.eqb_refl.
 Qed.
 
-Lemma eq_nat_refl n : eq_nat n n = true.
+Lemma eq_nat_refl n : eq_nat n n.
 Proof. by rewrite /eq_nat Nat.eqb_refl. Qed.
 
-Lemma eq_projection_refl i : eq_projection i i = true.
+Lemma eq_projection_refl i : eq_projection i i.
 Proof.
   destruct i as [[mind k] p].
   unfold eq_projection.
@@ -295,7 +295,7 @@ Close Scope string_scope.
 
 (** Combinators *)
 
-(** Forall combinators in Type to allow building them by *)
+(** Forall combinators in Type to allow building them by recursion *)
 Inductive All (A : Type) (P : A -> Type) : list A -> Type :=
     All_nil : All A P []
   | All_cons : forall (x : A) (l : list A),
@@ -306,10 +306,10 @@ Inductive Alli {A} (P : nat -> A -> Type) (n : nat) : list A -> Type :=
 | Alli_nil : Alli P n []
 | Alli_cons hd tl : P n hd -> Alli P (S n) tl -> Alli P n (hd :: tl).
 
-Inductive Forall2 {A B : Type} (R : A -> B -> Type) : list A -> list B -> Type :=
-  Forall2_nil : Forall2 R [] []
-| Forall2_cons : forall (x : A) (y : B) (l : list A) (l' : list B),
-    R x y -> Forall2 R l l' -> Forall2 R (x :: l) (y :: l').
+Inductive All2 {A B : Type} (R : A -> B -> Type) : list A -> list B -> Type :=
+  All2_nil : All2 R [] []
+| All2_cons : forall (x : A) (y : B) (l : list A) (l' : list B),
+    R x y -> All2 R l l' -> All2 R (x :: l) (y :: l').
 
 Inductive OnOne2 {A : Type} (P : A -> A -> Type) : list A -> list A -> Type :=
 | OnOne2_hd hd hd' tl : P hd hd' -> OnOne2 P (hd :: tl) (hd' :: tl)
@@ -388,28 +388,27 @@ Lemma map_def_id {t : Set} : map_def (@id t) (@id t) = id.
 Proof. extensionality p. now destruct p. Qed.
 Hint Rewrite @map_def_id @map_id : map.
 
-Lemma forall_map_spec {A B} {P : A -> Prop} {l} {f g : A -> B} :
-  Forall P l -> (forall x, P x -> f x = g x) ->
+Lemma forall_map_spec {A B} {l} {f g : A -> B} :
+  Forall (fun x => f x = g x) l <->
   map f l = map g l.
 Proof.
+  split.
   induction 1; simpl; trivial.
-  intros Heq. rewrite Heq //. f_equal; auto.
+  now rewrite IHForall H.
+  induction l => /= // [=] Ha Hl; constructor; auto.
 Qed.
 
 Lemma forall_map_id_spec {A} {P : A -> Prop} {l} {f : A -> A} :
-  Forall P l -> (forall x, P x -> f x = x) ->
-  map f l = l.
+  Forall (fun x => f x = x) l <-> map f l = l.
 Proof.
-  induction 1; simpl; trivial.
-  intros Heq. rewrite Heq //. f_equal; auto.
+  rewrite -{3}(map_id l). apply forall_map_spec.
 Qed.
 
-Lemma on_snd_spec {A B C} (P : B -> Prop) (f g : B -> C) (x : A * B) :
-  P (snd x) -> (forall x, P x -> f x = g x) ->
+Lemma on_snd_eq_spec {A B C} (f g : B -> C) (x : A * B) :
+  f (snd x) = g (snd x) <->
   on_snd f x = on_snd g x.
 Proof.
-  intros. destruct x. unfold on_snd. simpl.
-  now rewrite H0; auto.
+  case: x => /=; rewrite /on_snd /=. split; congruence.
 Qed.
 
 Lemma map_def_spec {A B : Set} (P P' : A -> Prop) (f f' g g' : A -> B) (x : def A) :
@@ -425,10 +424,9 @@ Lemma case_brs_map_spec {A B : Set} {P : A -> Prop} {l} {f g : A -> B} :
   tCaseBrsProp P l -> (forall x, P x -> f x = g x) ->
   map (on_snd f) l = map (on_snd g) l.
 Proof.
-  intros.
-  eapply (forall_map_spec H).
-  intros.
-  eapply on_snd_spec; eauto.
+  intros. red in H.
+  eapply forall_map_spec. eapply Forall_impl; eauto. simpl; intros.
+  apply on_snd_eq_spec; eauto.
 Qed.
 
 Lemma tfix_map_spec {A B : Set} {P P' : A -> Prop} {l} {f f' g g' : A -> B} :
@@ -437,175 +435,253 @@ Lemma tfix_map_spec {A B : Set} {P P' : A -> Prop} {l} {f f' g g' : A -> B} :
   map (map_def f f') l = map (map_def g g') l.
 Proof.
   intros.
-  eapply (forall_map_spec H).
+  eapply forall_map_spec. red in H. eapply Forall_impl; eauto. simpl.
   intros. destruct H2;
   eapply map_def_spec; eauto.
 Qed.
 
-Lemma Forall_forall_mix {A : Type} {P : A -> Prop} {p : A -> bool} {l : list A} :
-  Forall P l -> forallb p l = true -> Forall (fun x => P x /\ p x = true) l.
+
+Section Reverse_Induction.
+  Context {A : Type}.
+  Lemma rev_list_ind :
+    forall P:list A-> Type,
+      P [] ->
+        (forall (a:A) (l:list A), P (List.rev l) -> P (List.rev (a :: l))) ->
+        forall l:list A, P (List.rev l).
+    Proof.
+      induction l; auto.
+    Qed.
+
+    Theorem rev_ind :
+      forall P:list A -> Type,
+        P [] ->
+        (forall (x:A) (l:list A), P l -> P (l ++ [x])) -> forall l:list A, P l.
+    Proof.
+      intros.
+      generalize (rev_involutive l).
+      intros E; rewrite <- E.
+      apply (rev_list_ind P).
+      auto.
+
+      simpl.
+      intros.
+      apply (X0 a (List.rev l0)).
+      auto.
+    Qed.
+
+End Reverse_Induction.
+
+Lemma andb_and b b' : b && b' <-> b /\ b'.
+Proof. elim (@andP b b'); intuition. Qed.
+
+Lemma forallb_Forall {A} (p : pred A) l : Forall p l <-> forallb p l.
 Proof.
-  induction 1. constructor. simpl. rewrite andb_true_iff. intuition.
+  split.
+  induction 1; rewrite /= // H IHForall //.
+  induction l; rewrite /= //. move/andP => [pa pl].
+  constructor; auto.
 Qed.
+
+(** Generic strategy for dealing with Forall/forall, etc:
+
+    1) Move all boolean foralls into All/All2 (in the goal and the context).
+    2) Merge all context Foralls into one
+    3) Apply Forall implication
+    4) optionally simplify and call eauto.
+*)
 
 Lemma Forall_mix {A} (P Q : A -> Prop) : forall l, Forall P l -> Forall Q l -> Forall (fun x => P x /\ Q x) l.
 Proof.
   intros l Hl Hq. induction Hl; inv Hq; constructor; auto.
 Qed.
 
-Lemma forallb2_Forall2 {A : Type} {p : A -> A -> bool}
+Lemma forallb2_All2 {A : Type} {p : A -> A -> bool}
       {l l' : list A} :
-  forallb2 p l l' = true -> Forall2 (fun x y => p x y = true) l l'.
+  forallb2 p l l' -> All2 (fun x y => p x y) l l'.
 Proof.
   induction l in l' |- *; destruct l'; simpl; intros; try congruence.
   - constructor.
-  - constructor. revert H; rewrite andb_true_iff; intros [px pl]. auto.
-    apply IHl. revert H; rewrite andb_true_iff; intros [px pl]. auto.
+  - constructor. revert H; rewrite andb_and; intros [px pl]. auto.
+    apply IHl. revert H; rewrite andb_and; intros [px pl]. auto.
 Qed.
 
-Lemma Forall2_forallb2 {A : Type} {p : A -> A -> bool}
+Lemma All2_forallb2 {A : Type} {p : A -> A -> bool}
       {l l' : list A} :
-  Forall2 (fun x y => p x y = true) l l' -> forallb2 p l l' = true.
+  All2 (fun x y => p x y) l l' -> forallb2 p l l'.
 Proof.
   induction 1; simpl; intros; try congruence.
-  rewrite andb_true_iff. intuition auto.
+  rewrite andb_and. intuition auto.
 Qed.
-Require Import ssrbool.
+
 Lemma forallb2_app {A} (p : A -> A -> bool) l l' q q' :
-  forallb2 p l l' && forallb2 p q q' = true -> forallb2 p (l ++ q) (l' ++ q') = true.
+  forallb2 p l l' && forallb2 p q q' -> forallb2 p (l ++ q) (l' ++ q').
 Proof.
   induction l in l' |- *; destruct l'; simpl; try congruence.
   move=> /andP[/andP[pa pl] pq]. now rewrite pa IHl // pl pq.
 Qed.
 
-Lemma forallb2_forallb2 {A} (f : A -> A -> bool) g l l' :
-  (forall x y, f x y = true -> f (g x) (g y) = true) ->
-  forallb2 f l l' = true -> forallb2 f (map g l) (map g l') = true.
-Proof.
-  induction l in l' |- *; destruct l'; auto.
-  simpl; intros.
-  rewrite -> andb_true_iff in *. intuition.
+Lemma All2_map {A B C D} (R : C -> D -> Type) (f : A -> C) (g : B -> D) l l' :
+  All2 (fun x y => R (f x) (g y)) l l' -> All2 R (map f l) (map g l').
+Proof. induction 1; simpl; constructor; try congruence. Qed.
+
+Lemma All2_map_inv {A B C D} (R : C -> D -> Type) (f : A -> C) (g : B -> D) l l' :
+  All2 R (map f l) (map g l') -> All2 (fun x y => R (f x) (g y)) l l'.
+Proof. induction l in l' |- *; destruct l'; simpl;
+         move=> H;inv H; try constructor; try congruence. eauto.
 Qed.
 
-Lemma Forall2_List_Forall_mix {A : Type} {P : A -> Prop} {Q : A -> A -> Prop}
-      {l l' : list A} :
-    List.Forall P l -> Forall2 Q l l' -> Forall2 (fun x y => P x /\ Q x y) l l'.
-Proof.
-  induction 2; simpl; intros; constructor.
-  inv H; intuition auto.
-  apply IHX. inv H; intuition auto.
-Qed.
+(* Lemma All2_List_Forall_mix_left {A : Type} {P : A -> Prop} {Q : A -> A -> Prop} *)
+(*       {l l' : list A} : *)
+(*     Forall P l -> All2 Q l l' -> All2 (fun x y => P x /\ Q x y) l l'. *)
+(* Proof. *)
+(*   induction 2; simpl; intros; constructor. *)
+(*   inv H; intuition auto. *)
+(*   apply IHX. inv H; intuition auto. *)
+(* Qed. *)
 
-Lemma Forall2_List_Forall_mix_right {A : Type} {P : A -> Prop} {Q : A -> A -> Prop}
-      {l l' : list A} :
-    List.Forall P l' -> Forall2 Q l l' -> Forall2 (fun x y => P y /\ Q x y) l l'.
-Proof.
-  induction 2; simpl; intros; constructor.
-  inv H; intuition auto.
-  apply IHX. inv H; intuition auto.
-Qed.
+(* Lemma All2_List_Forall_mix_right {A : Type} {P : A -> Prop} {Q : A -> A -> Prop} *)
+(*       {l l' : list A} : *)
+(*     Forall P l' -> All2 Q l l' -> All2 (fun x y => P y /\ Q x y) l l'. *)
+(* Proof. *)
+(*   induction 2; simpl; intros; constructor. *)
+(*   inv H; intuition auto. *)
+(*   apply IHX. inv H; intuition auto. *)
+(* Qed. *)
 
-Lemma Forall2_Forall_mix {A : Set} {P : A -> Type} {Q : A -> A -> Type}
+Lemma All2_All_mix_left {A} {P : A -> Type} {Q : A -> A -> Type}
       {l l' : list A} :
-  All P l -> Forall2 Q l l' -> Forall2 (fun x y => (P x * Q x y)%type) l l'.
+  All P l -> All2 Q l l' -> All2 (fun x y => (P x * Q x y)%type) l l'.
 Proof.
   induction 2; simpl; intros; constructor.
   inv X; intuition auto.
   apply IHX0. inv X; intuition auto.
 Qed.
 
-Lemma Forall2_map {A B C D} (R : C -> D -> Type) (f : A -> C) (g : B -> D) l l' :
-  Forall2 (fun x y => R (f x) (g y)) l l' -> Forall2 R (map f l) (map g l').
-Proof. induction 1; simpl; constructor; try congruence. Qed.
+Lemma All2_All_mix_right {A} {P : A -> Type} {Q : A -> A -> Type}
+      {l l' : list A} :
+  All P l' -> All2 Q l l' -> All2 (fun x y => (Q x y * P y)%type) l l'.
+Proof.
+  induction 2; simpl; intros; constructor.
+  inv X; intuition auto.
+  apply IHX0. inv X; intuition auto.
+Qed.
 
-Lemma OnOne2_mix_Forall_left {A} {P : A -> A -> Prop} {Q : A -> Prop} {l l'} :
-  List.Forall Q l -> OnOne2 P l l' -> OnOne2 (fun x y => P x y /\ Q x) l l'.
+Lemma Forall_All {A : Type} (P : A -> Prop) l :
+  Forall P l -> All P l.
+Proof.
+  induction l; intros H; constructor; auto. inv H. auto.
+  apply IHl. inv H; auto.
+Qed.
+
+Lemma All_Forall {A : Type} (P : A -> Prop) l :
+  All P l -> Forall P l.
+Proof. induction 1; constructor; auto. Qed.
+
+Lemma forallb_All {A} (p : pred A) l : forallb p l -> All p l.
+Proof.
+  move/forallb_Forall. apply Forall_All.
+Qed.
+
+Lemma All_forallb {A} (p : pred A) l : All p l -> forallb p l.
+Proof.
+  move/All_Forall. apply forallb_Forall.
+Qed.
+
+Lemma OnOne2_All_mix_left {A} {P : A -> A -> Type} {Q : A -> Type} {l l'} :
+  All Q l -> OnOne2 P l l' -> OnOne2 (fun x y => (P x y * Q x)%type) l l'.
 Proof.
   intros H; induction 1; constructor; try inv H; intuition.
-  apply IHX. now inv H.
 Qed.
 
 Lemma OnOne2_app {A} (P : A -> A -> Type) l tl tl' : OnOne2 P tl tl' -> OnOne2 P (l ++ tl) (l ++ tl').
 Proof. induction l; simpl; try constructor; auto. Qed.
 
-Lemma Forall_firstn {A} {P : A -> Prop} {l} {n} : List.Forall P l -> List.Forall P (firstn n l).
+Lemma All_firstn {A} {P : A -> Type} {l} {n} : All P l -> All P (firstn n l).
 Proof. intros HPL; induction HPL in n |- * ; simpl; destruct n; try econstructor; eauto. Qed.
 
-Lemma Forall_skipn {A} {P : A -> Prop} {l} {n} : List.Forall P l -> List.Forall P (skipn n l).
+Lemma All_skipn {A} {P : A -> Type} {l} {n} : All P l -> All P (skipn n l).
 Proof. intros HPL; induction HPL in n |- * ; simpl; destruct n; try econstructor; eauto. Qed.
 
-Inductive nth_error_Spec {A} (l : list A) (n : nat) : option A -> Type :=
-| nth_error_Spec_Some x : nth_error l n = Some x -> n < length l -> nth_error_Spec l n (Some x)
-| nth_error_Spec_None : length l <= n -> nth_error_Spec l n None.
-
-Lemma nth_error_Some_length {A} {l : list A} {n t} : nth_error l n = Some t -> n < length l.
-Proof. rewrite <- nth_error_Some. destruct (nth_error l n); congruence. Qed.
-
-Lemma nth_error_spec {A} (l : list A) (n : nat) : nth_error_Spec l n (nth_error l n).
-Proof.
-  destruct nth_error eqn:Heq.
-  constructor; auto. now apply nth_error_Some_length in Heq.
-  constructor; auto. now apply nth_error_None in Heq.
-Qed.
-
-Require Import Arith.
-
-
-Lemma nth_error_app_left {A} (l l' : list A) n t : nth_error l n = Some t -> nth_error (l ++ l') n = Some t.
-Proof. induction l in n |- *; destruct n; simpl; try congruence. auto. Qed.
-
-Lemma nth_error_nil {A} n : nth_error (@nil A) n = None.
-Proof. destruct n; auto. Qed.
-Hint Rewrite @nth_error_nil.
-
-Lemma nth_error_forall {A} {P : A -> Prop} {l : list A} {n x} :
-  nth_error l n = Some x -> List.Forall P l -> P x.
-Proof.
-  intros Hnth HPl. induction HPl in n, Hnth |- *. destruct n; discriminate.
-  revert Hnth. destruct n. now intros [= ->].
-  intros H'; eauto.
-Qed.
-
-Lemma nth_error_all {A} {P : A -> Type} {l : list A} {n x} :
-  nth_error l n = Some x -> All P l -> P x.
-Proof.
-  intros Hnth HPl. induction HPl in n, Hnth |- *. destruct n; discriminate.
-  revert Hnth. destruct n. now intros [= ->].
-  intros H'; eauto.
-Qed.
-Require Import Arith.
-Lemma nth_error_alli {A} {P : nat -> A -> Type} {l : list A} {n x} {k} :
-  nth_error l n = Some x -> Alli P k l -> P (k + n) x.
-Proof.
-  intros Hnth HPl. induction HPl in n, Hnth |- *.
-  destruct n; discriminate.
-  revert Hnth. destruct n. intros [= ->]. now rewrite Nat.add_0_r.
-  intros H'; eauto. rewrite <- Nat.add_succ_comm. eauto.
-Qed.
-
-Lemma All_app {A} (P : A -> Type) l l' : All P (l ++ l') -> All P l * All P l'.
+Lemma All_app {A} {P : A -> Type} {l l'} : All P (l ++ l') -> All P l * All P l'.
 Proof.
   induction l; simpl; auto. intros. constructor; auto. constructor.
   intros. inv X. intuition auto. constructor; auto.
 Qed.
 
-Lemma All_mix {A} (P : A -> Type) (Q : A -> Type) l :
+Lemma All_app_inv {A} (P : A -> Type) l l' : All P l -> All P l' -> All P (l ++ l').
+Proof.
+  intros Hl Hl'. induction Hl. apply Hl'.
+  constructor; intuition auto.
+Qed.
+
+Lemma All_mix {A} {P : A -> Type} {Q : A -> Type} {l} :
   All P l -> All Q l -> All (fun x => (P x * Q x)%type) l.
 Proof. induction 1; intros Hq; inv Hq; constructor; auto. Qed.
 
-Lemma All_Forall {A} (P : A -> Type) (Q : A -> Prop) l :
-  (forall x, P x -> Q x) ->
-  All P l -> Forall Q l.
-Proof. induction 2; constructor; auto. Qed.
+Lemma All2_All_left {A B} {P : A -> B -> Type} {Q : A -> Type} {l l'} :
+  All2 P l l' ->
+  (forall x y, P x y -> Q x) ->
+  All Q l.
+Proof.
+  intros HF H. induction HF; constructor; eauto.
+Qed.
 
-Lemma Alli_mix {A} (P : nat -> A -> Type) (Q : nat -> A -> Type) n l :
+Lemma All2_All_right {A B} {P : A -> B -> Type} {Q : B -> Type} {l l'} :
+  All2 P l l' ->
+  (forall x y, P x y -> Q y) ->
+  All Q l'.
+Proof.
+  intros HF H. induction HF; constructor; eauto.
+Qed.
+
+Lemma All2_right {A B} {P : B -> Type} {l : list A} {l'} :
+  All2 (fun x y => P y) l l' -> All P l'.
+Proof.
+  induction 1; constructor; auto.
+Qed.
+
+Hint Constructors All All2.
+
+Lemma All_rev_map {A B} (P : A -> Prop) f (l : list B) : All (compose P f) l -> All P (rev_map f l).
+Proof. induction 1. constructor. rewrite rev_map_cons. apply All_app_inv; auto. Qed.
+
+Lemma All_rev {A} (P : A -> Prop) (l : list A) : All P l -> All P (List.rev l).
+Proof.
+  induction l using rev_ind. constructor.
+  intros. rewrite rev_app_distr. simpl. apply All_app in X as [Alll Allx]. inv Allx.
+  constructor; intuition eauto.
+Qed.
+
+Lemma All_rev_inv {A} (P : A -> Prop) (l : list A) : All P (List.rev l) -> All P l.
+Proof.
+  induction l using rev_ind. constructor.
+  intros. rewrite rev_app_distr in X. simpl.
+  apply All_app in X as [Allx Alll]. inv Allx.
+   apply All_app_inv; intuition eauto.
+Qed.
+
+Lemma All_impl {A} {P Q} {l : list A} : All P l -> (forall x, P x -> Q x) -> All Q l.
+Proof. induction 1; try constructor; intuition auto. Qed.
+
+Lemma Alli_impl {A} {P Q} (l : list A) {n} : Alli P n l -> (forall n x, P n x -> Q n x) -> Alli Q n l.
+Proof. induction 1; try constructor; intuition auto. Qed.
+
+Lemma All_map {A B} {P : B -> Type} {f : A -> B} {l : list A} :
+  All (compose P f) l -> All P (map f l).
+Proof. induction 1; constructor; auto. Qed.
+
+Lemma All_map_inv {A B} (P : B -> Prop) (f : A -> B) l : All P (map f l) -> All (compose P f) l.
+Proof. induction l; intros Hf; inv Hf; try constructor; eauto. Qed.
+
+Lemma Alli_mix {A} {P : nat -> A -> Type} {Q : nat -> A -> Type} {n l} :
   Alli P n l -> Alli Q n l -> Alli (fun n x => (P n x * Q n x)%type) n l.
 Proof. induction 1; intros Hq; inv Hq; constructor; auto. Qed.
 
-Lemma Alli_Forall {A} (P : nat -> A -> Type) (Q : A -> Prop) l n :
+Lemma Alli_All {A} {P : nat -> A -> Type} {Q : A -> Type} {l n} :
+  Alli P n l ->
   (forall n x, P n x -> Q x) ->
-  Alli P n l -> Forall Q l.
-Proof. induction 2; constructor; eauto. Qed.
+  All Q l.
+Proof. induction 1; constructor; eauto. Qed.
 
 Lemma Alli_app {A} (P : nat -> A -> Type) n l l' : Alli P n (l ++ l') -> Alli P n l * Alli P (length l + n) l'.
 Proof.
@@ -615,49 +691,98 @@ Proof.
   eapply IHl; eauto.
 Qed.
 
-Ltac merge_Forall := unfold tFixProp, tCaseBrsProp in *;
+Ltac toProp :=
   repeat match goal with
-  | H : Forall _ ?x, H' : Forall _ ?x |- _ =>
-    apply (Forall_mix _ _ _ H) in H'; clear H
+  | H : _ && _ |- _ => apply andb_and in H; destruct H
+  | |- _ && _ => apply andb_and
+  end.
+
+Ltac toAll :=
+  match goal with
+  | H : is_true (forallb _ _) |- _ => apply forallb_All in H
+
+  | |- is_true (forallb _ _) => apply All_forallb
+
+  | H : Forall _ ?x |- _ => apply Forall_All in H
+
+  | |- Forall _ _ => apply All_Forall
+
+  | H : is_true (forallb2 _ _ _) |- _ => apply forallb2_All2 in H
+
+  | |- is_true (forallb2 _ _ _) => apply All2_forallb2
+
   | H : All _ ?x, H' : All _ ?x |- _ =>
-    apply (All_mix _ _ _ H) in H'; clear H
+    apply (All_mix H) in H'; clear H
+
   | H : Alli _ _ ?x, H' : Alli _ _ ?x |- _ =>
-    apply (Alli_mix _ _ _ _ H) in H'; clear H
-  | H : Forall _ ?x, H' : forallb _ ?x = _ |- _ =>
-    eapply (Forall_forall_mix H) in H'; clear H
-  | H : forallb2 _ _ _ = _ |- _ => apply forallb2_Forall2 in H
-  | |- forallb2 _ _ _ = _ => apply Forall2_forallb2
-  | H : Forall _ ?x, H' : Forall2 _ ?x _  |- _ =>
-    apply (Forall2_List_Forall_mix H) in H'; clear H
-  | H : Forall _ ?x, H' : Forall2 _ _ ?x  |- _ =>
-    apply (Forall2_List_Forall_mix_right H) in H'; clear H
-  | |- Forall2 _ (map _ _) (map _ _) => apply Forall2_map
-  | H : Forall _ ?x, H' : is_true (forallb _ ?x) |- _ =>
-    eapply (Forall_forall_mix H) in H'; clear H
+    apply (Alli_mix H) in H'; clear H
+
+  | H : All _ ?x, H' : All2 _ ?x _  |- _ =>
+    apply (All2_All_mix_left H) in H'; clear H
+
+  | H : All _ ?x, H' : All2 _ _ ?x  |- _ =>
+    apply (All2_All_mix_right H) in H'; clear H
+
+  | |- All _ (map _ _) => apply All_map
+
+  | H : All _ (map _ _) |- _ => apply All_map_inv in H
+
+  | |- All _ (rev_map _ _) => apply All_rev_map
+
+  | |- All _ (List.rev _) => apply All_rev
+
+  | |- All2 _ (map _ _) (map _ _) => apply All2_map
+  end.
+
+Ltac merge_All :=
+  unfold tFixProp, tCaseBrsProp in *;
+  repeat toAll.
+
+
+Lemma All_map_eq {A B} {l} {f g : A -> B} :
+  All (fun x => f x = g x) l ->
+  map f l = map g l.
+Proof.
+  induction 1; simpl; trivial.
+  now rewrite IHX p.
+Qed.
+
+Lemma All_map_id {A} {l} {f : A -> A} :
+  All (fun x => f x = x) l ->
+  map f l = l.
+Proof.
+  induction 1; simpl; trivial.
+  now rewrite IHX p.
+Qed.
+
+Ltac All_map :=
+  match goal with
+    |- map _ _ = map _ _ => apply All_map_eq
+  | |- map _ _ = _ => apply All_map_id
   end.
 
 Lemma forall_forallb_map_spec {A B : Type} {P : A -> Prop} {p : A -> bool}
       {l : list A} {f g : A -> B} :
-    Forall P l -> forallb p l = true ->
-    (forall x : A, P x -> p x = true -> f x = g x) -> map f l = map g l.
+    Forall P l -> forallb p l ->
+    (forall x : A, P x -> p x -> f x = g x) -> map f l = map g l.
 Proof.
   induction 1; simpl; trivial.
-  rewrite andb_true_iff. intros [px pl] Hx.
+  rewrite andb_and. intros [px pl] Hx.
   f_equal. now apply Hx. now apply IHForall.
 Qed.
 
 Lemma forall_forallb_forallb_spec {A : Type} {P : A -> Prop} {p : A -> bool}
       {l : list A} {f : A -> bool} :
-    Forall P l -> forallb p l = true ->
-    (forall x : A, P x -> p x = true -> f x = true) -> forallb f l = true.
+    Forall P l -> forallb p l ->
+    (forall x : A, P x -> p x -> f x) -> forallb f l.
 Proof.
   induction 1; simpl; trivial.
-  rewrite !andb_true_iff. intros [px pl] Hx. eauto.
+  rewrite !andb_and. intros [px pl] Hx. eauto.
 Qed.
 
 Lemma on_snd_test_spec {A B C} (P : B -> Prop) (p : B -> bool) (f g : B -> C) (x : A * B) :
-  P (snd x) -> (forall x, P x -> p x = true -> f x = g x) ->
-  test_snd p x = true ->
+  P (snd x) -> (forall x, P x -> p x -> f x = g x) ->
+  test_snd p x ->
   on_snd f x = on_snd g x.
 Proof.
   intros. destruct x. unfold on_snd. simpl.
@@ -665,22 +790,22 @@ Proof.
 Qed.
 
 Lemma map_def_test_spec {A B : Set}
-      (P P' : A -> Prop) p p' (f f' g g' : A -> B) (x : def A) :
-  P x.(dtype) -> P' x.(dbody) -> (forall x, P x -> p x = true -> f x = g x) ->
-  (forall x, P' x -> p' x = true -> f' x = g' x) ->
-  test_def p p' x = true ->
+      (P P' : A -> Prop) (p p' : pred A) (f f' g g' : A -> B) (x : def A) :
+  P x.(dtype) -> P' x.(dbody) -> (forall x, P x -> p x -> f x = g x) ->
+  (forall x, P' x -> p' x -> f' x = g' x) ->
+  test_def p p' x ->
   map_def f f' x = map_def g g' x.
 Proof.
   intros. destruct x. unfold map_def. simpl.
-  unfold test_def in H3; simpl in H3. rewrite -> andb_true_iff in H3. intuition.
+  unfold test_def in H3; simpl in H3. rewrite -> andb_and in H3. intuition.
   rewrite !H1 // !H2 //; intuition auto.
 Qed.
 
 Lemma case_brs_forallb_map_spec {A B : Set} {P : A -> Prop} {p : A -> bool}
       {l} {f g : A -> B} :
   tCaseBrsProp P l ->
-  forallb (test_snd p) l = true ->
-  (forall x, P x -> p x = true -> f x = g x) ->
+  forallb (test_snd p) l ->
+  (forall x, P x -> p x -> f x = g x) ->
   map (on_snd f) l = map (on_snd g) l.
 Proof.
   intros.
@@ -691,9 +816,9 @@ Qed.
 
 Lemma tfix_forallb_map_spec {A B : Set} {P P' : A -> Prop} {p p'} {l} {f f' g g' : A -> B} :
   tFixProp P P' l ->
-  forallb (test_def p p') l = true ->
-  (forall x, P x -> p x = true -> f x = g x) ->
-  (forall x, P' x -> p' x = true -> f' x = g' x) ->
+  forallb (test_def p p') l ->
+  (forall x, P x -> p x -> f x = g x) ->
+  (forall x, P' x -> p' x -> f' x = g' x) ->
   map (map_def f f') l = map (map_def g g') l.
 Proof.
   intros.
@@ -702,12 +827,12 @@ Proof.
   eapply map_def_test_spec; eauto.
 Qed.
 
-Lemma Forall_forallb {A} P (l : list A) p :
+Lemma Forall_forallb {A} P (l : list A) (p : pred A) :
   Forall P l ->
-  (forall x, P x -> p x = true) ->
-  forallb p l = true.
+  (forall x, P x -> p x) ->
+  forallb p l.
 Proof.
-  induction 1 in p |- *; unfold compose; simpl; rewrite ?andb_true_iff;
+  induction 1 in p |- *; unfold compose; simpl; rewrite ?andb_and;
     intuition auto.
 Qed.
 
@@ -753,51 +878,25 @@ Proof.
   induction 1; constructor; auto.
 Qed.
 
-Lemma Forall2_impl {A B} {P Q : A -> B -> Type} {l l'} :
-    Forall2 P l l' ->
+Lemma All2_impl {A B} {P Q : A -> B -> Type} {l l'} :
+    All2 P l l' ->
     (forall x y, P x y -> Q x y) ->
-    Forall2 Q l l'.
+    All2 Q l l'.
 Proof.
   induction 1; constructor; auto.
 Qed.
 
-Lemma Forall_app {A} (P : A -> Prop) l l' : List.Forall P (l ++ l') -> List.Forall P l /\ List.Forall P l'.
+Lemma Forall_app {A} (P : A -> Prop) l l' : Forall P (l ++ l') -> Forall P l /\ Forall P l'.
 Proof.
   induction l; intros H. split; try constructor. apply H.
   inversion_clear H. split; intuition auto.
 Qed.
 
-Lemma Forall_app_inv {A} (P : A -> Prop) l l' : List.Forall P l /\ List.Forall P l' -> List.Forall P (l ++ l').
-  intros [Hl Hl']. induction Hl. apply Hl'.
-  constructor; intuition auto.
-Qed.
 
 Lemma firstn_map {A B} n (f : A -> B) l : firstn n (map f l) = map f (firstn n l).
 Proof.
   revert l; induction n. reflexivity.
   destruct l; simpl in *; congruence.
-Qed.
-
-Lemma Forall2_Forall_left {A B} {P : A -> B -> Type} {Q : A -> Prop} {l l'} :
-  Forall2 P l l' ->
-  (forall x y, P x y -> Q x) ->
-  List.Forall Q l.
-Proof.
-  intros HF H. induction HF; constructor; eauto.
-Qed.
-
-Lemma Forall2_Forall_right {A B} {P : A -> B -> Type} {Q : B -> Prop} {l l'} :
-  Forall2 P l l' ->
-  (forall x y, P x y -> Q y) ->
-  List.Forall Q l'.
-Proof.
-  intros HF H. induction HF; constructor; eauto.
-Qed.
-
-Lemma Forall2_right {A B} {P : B -> Prop} {l : list A} {l'} :
-  Forall2 (fun x y => P y) l l' -> List.Forall (fun x => P x) l'.
-Proof.
-  induction 1; constructor; auto.
 Qed.
 
 Lemma All_safe_nth {A} {P : A -> Type} {Γ n} (isdecl : n < length Γ) : All P Γ ->
@@ -808,25 +907,7 @@ Proof.
   simpl in *. eapply IHX.
 Qed.
 
-Lemma Forall_rev_map {A B} (P : A -> Prop) f (l : list B) : Forall (compose P f) l -> Forall P (rev_map f l).
-Proof. induction 1. constructor. rewrite rev_map_cons. apply Forall_app_inv. split; auto. Qed.
-
-Lemma Forall_rev {A} (P : A -> Prop) (l : list A) : Forall P l -> Forall P (List.rev l).
-Proof.
-  induction l using rev_ind. constructor.
-  intros. rewrite rev_app_distr. apply Forall_app_inv. apply Forall_app in H. intuition auto.
-Qed.
-
 Definition size := nat.
-Lemma All_impl {A} {P Q} (l : list A) : All P l -> (forall x, P x -> Q x) -> All Q l.
-Proof. induction 1; try constructor; intuition auto. Qed.
-
-Lemma Alli_impl {A} {P Q} (l : list A) {n} : Alli P n l -> (forall n x, P n x -> Q n x) -> Alli Q n l.
-Proof. induction 1; try constructor; intuition auto. Qed.
-
-Lemma All_map {A B} (P : B -> Type) (f : A -> B) (l : list A) :
-  All (compose P f) l -> All P (map f l).
-Proof. induction 1; constructor; auto. Qed.
 
 (* Lemma Alli_mapi {A B} (P : nat -> B -> Type) (f : nat -> A -> B) (l : list A) n : *)
 (*   Alli (fun n x => P n (f n x)) n l -> Alli P n (mapi f l). *)
@@ -852,23 +933,24 @@ End Alli_size.
 
 Section All2_size.
   Context {A} (P : A -> A -> Type) (fn : forall x1 x2, P x1 x2 -> size).
-  Fixpoint all2_size {l1 l2 : list A} (f : Forall2 P l1 l2) : size :=
+  Fixpoint all2_size {l1 l2 : list A} (f : All2 P l1 l2) : size :=
   match f with
-  | Forall2_nil => 0
-  | Forall2_cons x y l l' rxy rll' => fn _ _ rxy + all2_size rll'
+  | All2_nil => 0
+  | All2_cons x y l l' rxy rll' => fn _ _ rxy + all2_size rll'
   end.
 End All2_size.
 
 Ltac close_Forall :=
   match goal with
-  | H : Forall _ _ _ |- Forall _ _ _ => apply (Forall_impl H)
-  | H : Forall2 _ _ _ |- Forall2 _ _ _ => apply (Forall2_impl H)
-  | H : Forall2 _ _ _ |- Forall _ _ _ =>
-    apply (Forall2_Forall_left H) || apply (Forall2_Forall_right H)
+  | H : Forall _ _ |- Forall _ _ => apply (Forall_impl H); clear H; simpl
+  | H : All _ _ |- All _ _ => apply (All_impl H); clear H; simpl
+  | H : All2 _ _ _ |- All2 _ _ _ => apply (All2_impl H); clear H; simpl
+  | H : All2 _ _ _ |- All _ _ =>
+    (apply (All2_All_left H) || apply (All2_All_right H)); clear H; simpl
   end.
 
-Lemma Forall2_non_nil {A B} (P : A -> B -> Prop) (l : list A) (l' : list B) :
-  Forall2 P l l' -> l <> nil -> l' <> nil.
+Lemma All2_non_nil {A B} (P : A -> B -> Prop) (l : list A) (l' : list B) :
+  All2 P l l' -> l <> nil -> l' <> nil.
 Proof.
   induction 1; congruence.
 Qed.
@@ -920,6 +1002,10 @@ Proof.
   now intros [=].
 Qed.
 
+Inductive nth_error_Spec {A} (l : list A) (n : nat) : option A -> Type :=
+| nth_error_Spec_Some x : nth_error l n = Some x -> n < length l -> nth_error_Spec l n (Some x)
+| nth_error_Spec_None : length l <= n -> nth_error_Spec l n None.
+
 Lemma mapi_rec_eqn {A B} (f : nat -> A -> B) (l : list A) a n :
   mapi_rec f (a :: l) n = f n a :: mapi_rec f l (S n).
 Proof. simpl. f_equal. Qed.
@@ -939,6 +1025,48 @@ Lemma nth_error_mapi {A B} (f : nat -> A -> B) n l :
 Proof.
   unfold mapi; rewrite nth_error_mapi_rec.
   now rewrite -> Nat.add_0_r.
+Qed.
+
+Lemma nth_error_Some_length {A} {l : list A} {n t} : nth_error l n = Some t -> n < length l.
+Proof. rewrite <- nth_error_Some. destruct (nth_error l n); congruence. Qed.
+
+Lemma nth_error_spec {A} (l : list A) (n : nat) : nth_error_Spec l n (nth_error l n).
+Proof.
+  destruct nth_error eqn:Heq.
+  constructor; auto. now apply nth_error_Some_length in Heq.
+  constructor; auto. now apply nth_error_None in Heq.
+Qed.
+
+Lemma nth_error_app_left {A} (l l' : list A) n t : nth_error l n = Some t -> nth_error (l ++ l') n = Some t.
+Proof. induction l in n |- *; destruct n; simpl; try congruence. auto. Qed.
+
+Lemma nth_error_nil {A} n : nth_error (@nil A) n = None.
+Proof. destruct n; auto. Qed.
+Hint Rewrite @nth_error_nil.
+
+Lemma nth_error_forall {A} {P : A -> Prop} {l : list A} {n x} :
+  nth_error l n = Some x -> Forall P l -> P x.
+Proof.
+  intros Hnth HPl. induction HPl in n, Hnth |- *. destruct n; discriminate.
+  revert Hnth. destruct n. now intros [= ->].
+  intros H'; eauto.
+Qed.
+
+Lemma nth_error_all {A} {P : A -> Type} {l : list A} {n x} :
+  nth_error l n = Some x -> All P l -> P x.
+Proof.
+  intros Hnth HPl. induction HPl in n, Hnth |- *. destruct n; discriminate.
+  revert Hnth. destruct n. now intros [= ->].
+  intros H'; eauto.
+Qed.
+Require Import Arith.
+Lemma nth_error_alli {A} {P : nat -> A -> Type} {l : list A} {n x} {k} :
+  nth_error l n = Some x -> Alli P k l -> P (k + n) x.
+Proof.
+  intros Hnth HPl. induction HPl in n, Hnth |- *.
+  destruct n; discriminate.
+  revert Hnth. destruct n. intros [= ->]. now rewrite Nat.add_0_r.
+  intros H'; eauto. rewrite <- Nat.add_succ_comm. eauto.
 Qed.
 
 Fixpoint chop {A} (n : nat) (l : list A) :=
@@ -963,7 +1091,7 @@ Qed.
 Definition on_pi2 {A B C} (f : B -> B) (p : A * B * C) : A * B * C :=
   (fst (fst p), f (snd (fst p)), snd p).
 
-Lemma All_map_id {A} {P : A -> Type} {l} {f} :
+Lemma All_map_id' {A} {P : A -> Type} {l} {f} :
   All P l ->
   (forall x, P x -> f x = x) ->
   map f l = l.
@@ -1078,8 +1206,8 @@ Qed.
 Lemma rev_mapi_rec {A B} (f : nat -> A -> B) (l : list A) n k : k <= n ->
   List.rev (mapi_rec f l (n - k)) = mapi_rec (fun k x => f (Nat.pred (length l) + n - k) x) (List.rev l) k.
 Proof.
-  unfold mapi.
-  induction l in n, k |- * using rev_ind; simpl; try congruence.
+  unfold mapi. revert n k.
+  induction l using rev_ind; simpl; try congruence.
   intros. rewrite rev_unit. simpl.
   rewrite mapi_rec_app rev_app_distr; simpl. rewrite IHl; auto. simpl.
   rewrite app_length. simpl. f_equal. f_equal. lia. rewrite mapi_rec_Sk.
@@ -1097,8 +1225,8 @@ Qed.
 Lemma mapi_rec_rev {A B} (f : nat -> A -> B) (l : list A) n :
   mapi_rec f (List.rev l) n = List.rev (mapi (fun k x => f (length l + n - S k) x) l).
 Proof.
-  unfold mapi.
-  induction l in n |- * using rev_ind; simpl; try congruence.
+  unfold mapi. revert n.
+  induction l using rev_ind; simpl; try congruence.
   intros. rewrite rev_unit. simpl.
   rewrite IHl mapi_rec_app.
   simpl. rewrite rev_unit. f_equal.
@@ -1129,40 +1257,40 @@ Qed.
 Lemma forallb_map {A B} (f : A -> B) (l : list A) p :
   forallb p (map f l) = forallb (compose p f) l.
 Proof.
-  induction l in p, f |- *; unfold compose; simpl; rewrite ?andb_true_iff;
+  induction l in p, f |- *; unfold compose; simpl; rewrite ?andb_and;
     intuition (f_equal; auto). apply IHl.
 Qed.
 
-Lemma All_forallb {A} P (l : list A) p :
+Lemma All_forallb' {A} P (l : list A) (p : pred A) :
   All P l ->
-  (forall x, P x -> p x = true) ->
-  forallb p l = true.
+  (forall x, P x -> p x) ->
+  forallb p l.
 Proof.
-  induction 1 in p |- *; unfold compose; simpl; rewrite ?andb_true_iff;
+  induction 1 in p |- *; unfold compose; simpl; rewrite ?andb_and;
     intuition auto.
 Qed.
 
-Lemma forallb_Forall {A} (P : A -> Prop) (l : list A) p :
-  forallb p l = true ->
-  (forall x, p x = true -> P x) ->
+Lemma forallb_Forall' {A} (P : A -> Prop) (l : list A) p :
+  forallb p l ->
+  (forall x, p x -> P x) ->
   Forall P l.
 Proof.
   induction l in p |- *; unfold compose; simpl. constructor.
-  intros. constructor; eauto; rewrite -> andb_true_iff in H; intuition eauto.
+  intros. constructor; eauto; rewrite -> andb_and in H; intuition eauto.
 Qed.
 
 Lemma forallb_skipn {A} (p : A -> bool) n l :
-  forallb p l = true ->
-  forallb p (skipn n l) = true.
+  forallb p l ->
+  forallb p (skipn n l).
 Proof.
   induction l in n |- *; destruct n; simpl; try congruence.
-  intros. apply IHl. rewrite -> andb_true_iff in H; intuition.
+  intros. apply IHl. rewrite -> andb_and in H; intuition.
 Qed.
 
 Lemma forallb_rev {A} (p : A -> bool) l :
   forallb p (List.rev l) = forallb p l.
 Proof.
-  induction l using rev_ind in |- *; simpl; try congruence.
+  induction l using rev_ind; simpl; try congruence.
   rewrite rev_unit forallb_app. simpl. rewrite <- IHl.
   now rewrite andb_comm andb_true_r.
 Qed.
@@ -1175,10 +1303,10 @@ Proof.
   induction 1; simpl; intuition (f_equal; auto).
 Qed.
 
-Lemma forallb2_length {A} (p : A -> A -> bool) l l' : forallb2 p l l' = true -> length l = length l'.
+Lemma forallb2_length {A} (p : A -> A -> bool) l l' : forallb2 p l l' -> length l = length l'.
 Proof.
   induction l in l' |- *; destruct l'; simpl; try congruence.
-  rewrite !andb_true_iff. intros [Hp Hl]. erewrite IHl; eauto.
+  rewrite !andb_and. intros [Hp Hl]. erewrite IHl; eauto.
 Qed.
 
 Definition arities_context (l : list one_inductive_body) :=
@@ -1483,33 +1611,3 @@ Proof.
   case E' : map_option_out => [b'|]; try congruence.
   move=> [= <-]. now rewrite (IHHa _ E').
 Qed.
-
-Section Reverse_Induction.
-  Context {A : Type}.
-  Lemma rev_list_ind :
-    forall P:list A-> Type,
-      P [] ->
-        (forall (a:A) (l:list A), P (List.rev l) -> P (List.rev (a :: l))) ->
-        forall l:list A, P (List.rev l).
-    Proof.
-      induction l; auto.
-    Qed.
-
-    Theorem rev_ind :
-      forall P:list A -> Type,
-        P [] ->
-        (forall (x:A) (l:list A), P l -> P (l ++ [x])) -> forall l:list A, P l.
-    Proof.
-      intros.
-      generalize (rev_involutive l).
-      intros E; rewrite <- E.
-      apply (rev_list_ind P).
-      auto.
-
-      simpl.
-      intros.
-      apply (X0 a (List.rev l0)).
-      auto.
-    Qed.
-
-End Reverse_Induction.
